

Úkol 4

4.2.1

(3) seznam $B_3 = \left(\begin{pmatrix} 1 \\ 4 \\ 3 \end{pmatrix}, \begin{pmatrix} 1 \\ 0 \\ 0 \end{pmatrix}, \begin{pmatrix} 4 \\ 8 \\ 6 \end{pmatrix} \right)$

Není uspořádanou bází lin. prostoru \mathbb{R}^3 !

protože:
$$\begin{pmatrix} 4 \\ 8 \\ 6 \end{pmatrix} = 2 \cdot \begin{pmatrix} 1 \\ 4 \\ 3 \end{pmatrix} + 2 \cdot \begin{pmatrix} 1 \\ 0 \\ 0 \end{pmatrix}$$

vektory nejsou lineárně nezávislé

Úkol 5

5.2.2

(1) dosadím bod $\begin{pmatrix} \cosh t \\ \sinh t \end{pmatrix}$ do $x^2 - y^2 = 1, x > 0$

$$(\cosh t)^2 - (\sinh t)^2 = 1$$

$$\frac{(e^t + e^{-t})^2}{4} - \frac{(e^t - e^{-t})^2}{4} = 1$$

~~$$\frac{e^{2t} + e^{-2t}}{4} - \frac{e^{2t} - e^{-2t}}{4} = 1$$~~

$$\frac{(e^{2t} + 2 + e^{-2t})}{4} - \frac{(e^{2t} - 2 + e^{-2t})}{4} = 1$$

$$\frac{e^{2t} + 2 + e^{-2t} - e^{2t} + 2 - e^{-2t}}{4} = 1$$

$$\frac{4}{4} = 1, \text{ pro } \cosh t > 0 \quad \square$$

(2)

$$H_t \cdot H_u = \begin{pmatrix} \cosh t & \sinh t \\ \sinh t & \cosh t \end{pmatrix} \cdot \begin{pmatrix} \cosh u & \sinh u \\ \sinh u & \cosh u \end{pmatrix} =$$

$$= \begin{pmatrix} \cosh t \cdot \cosh u + \sinh t \cdot \sinh u & \cosh t \cdot \sinh u + \sinh t \cdot \cosh u \\ \sinh t \cdot \cosh u + \cosh t \cdot \sinh u & \sinh t \cdot \sinh u + \cosh t \cdot \cosh u \end{pmatrix} =$$

$$= \begin{pmatrix} \frac{e^t + e^{-t}}{2} \cdot \frac{e^u + e^{-u}}{2} + \frac{e^t - e^{-t}}{2} \cdot \frac{e^u - e^{-u}}{2} & \frac{e^t + e^{-t}}{2} \cdot \frac{e^u - e^{-u}}{2} + \frac{e^t - e^{-t}}{2} \cdot \frac{e^u + e^{-u}}{2} \\ \frac{e^t - e^{-t}}{2} \cdot \frac{e^u + e^{-u}}{2} + \frac{e^t + e^{-t}}{2} \cdot \frac{e^u - e^{-u}}{2} & \frac{e^t - e^{-t}}{2} \cdot \frac{e^u - e^{-u}}{2} + \frac{e^t + e^{-t}}{2} \cdot \frac{e^u + e^{-u}}{2} \end{pmatrix} =$$

$$= \begin{pmatrix} \frac{e^t \cdot e^u + e^{-t} \cdot e^u}{2} & \frac{e^t \cdot e^u - e^{-t} \cdot e^u}{2} \\ \frac{e^t \cdot e^u - e^{-t} \cdot e^u}{2} & \frac{e^t \cdot e^u + e^{-t} \cdot e^u}{2} \end{pmatrix} = H_{t+u} = \begin{pmatrix} \frac{e^{u+t} + e^{u-t}}{2} & \frac{e^{u+t} - e^{u-t}}{2} \\ \frac{e^{u+t} - e^{u-t}}{2} & \frac{e^{u+t} + e^{u-t}}{2} \end{pmatrix} =$$

$$= H_{u+t} \quad \square$$

$$(e^t + e^{-t})(e^u + e^{-u}) = e^t \cdot e^u + e^{-t} \cdot e^u - e^t \cdot e^{-u} - e^{-t} \cdot e^{-u}$$

$$(e^t - e^{-t})(e^u - e^{-u}) = e^t \cdot e^u - e^{-t} \cdot e^u + e^t \cdot e^{-u} + e^{-t} \cdot e^{-u} \quad \oplus$$

$$\underline{2e^t \cdot e^u + 2e^{-t} \cdot e^{-u}}$$

$$(e^t + e^{-t})(e^u - e^{-u}) = e^t \cdot e^u + e^{-t} \cdot e^u - e^t \cdot e^{-u} - e^{-t} \cdot e^{-u}$$

$$(e^t - e^{-t})(e^u + e^{-u}) = e^t \cdot e^u - e^{-t} \cdot e^u + e^t \cdot e^{-u} - e^{-t} \cdot e^{-u} \quad \oplus$$

$$\underline{2e^t \cdot e^u - 2e^{-t} \cdot e^{-u}}$$